Proved topological sort and draft variables assignment

template-coq/theories/common/sGraph.v
@@ -61,6 +61,132 @@ Module WeightedGraphExt (V: UsualOrderedTypeWithLeibniz) (VSet : MSetList.SWithL
       (forall e, EdgeSet.In e (E G) -> e..s <> e..t).
   End self_loops.
 
+  Section Stuff.
+    Context (G : t).
+
+    Definition Partition (total part1 part2 part3 : VSet.t) : Prop :=
+      VSet.union part1 (VSet.union part2 part3) = total /\
+      VSet.Empty (VSet.inter part1 part2) /\
+      VSet.Empty (VSet.inter part2 part3) /\
+      VSet.Empty (VSet.inter part3 part1).
+
+    Lemma partition_move_21 total v s l x : VSet.In x s -> Partition total v s l ->
+      Partition total (VSet.add x v) (VSet.remove x s) l.
+    Proof.
+      intros H [[=<-] [inter12 [inter23 inter31]]].
+      repeat split; [apply VSet.eq_leibniz| | |]; intro y.
+      - repeat rewrite VSet.union_spec.
+        rewrite VSet.add_spec. rewrite VSet.remove_spec. split.
+        + intros [[H3%V.eq_leibniz|?]|[[? _]|?]];
+            [right;left;by rewrite H3|now left|now right;left|right; now right].
+        + intros H3. destruct (V.eq_dec y x); [now left;left|].
+          destruct H3 as [?|[?|?]]; [now left;right|now right;left|now right;right].
+      - rewrite VSet.inter_spec VSet.add_spec VSet.remove_spec.
+        intros [[?|?] [? ?]]; [contradiction|]. apply (inter12 y).
+        now rewrite VSet.inter_spec.
+      - rewrite VSet.inter_spec VSet.remove_spec.
+        intros [[? _] ?]. apply (inter23 y). now rewrite VSet.inter_spec.
+      - rewrite VSet.inter_spec VSet.add_spec. intros [? [H3|?]].
+        + apply (inter23 y). rewrite VSet.inter_spec.
+          split; [by rewrite H3|assumption].
+        + apply (inter31 y). now rewrite VSet.inter_spec.
+    Qed.
+
+    Lemma partition_move_23 total v s l x : VSet.In x s -> Partition total v s l ->
+      Partition total v (VSet.remove x s) (VSet.add x l).
+    Proof.
+      intros H [[=<-] [inter12 [inter23 inter31]]].
+      repeat split; [apply VSet.eq_leibniz| | |]; intro y.
+      - repeat rewrite VSet.union_spec. rewrite VSet.add_spec VSet.remove_spec.
+        split.
+        + intros [?|[[? _]|[?|?]]];
+          [by left|by right;left|by right;left;rewrite H0|by right;right].
+        + intros H0. destruct (V.eq_dec y x); [now right;right;left|].
+          destruct H0 as [?|[?|?]]; [by left|by right;left|by right;right;right].
+      - rewrite VSet.inter_spec VSet.remove_spec.
+        intros [? [? ?]]. apply (inter12 y). by rewrite VSet.inter_spec.
+      - rewrite VSet.inter_spec VSet.add_spec VSet.remove_spec.
+        intros [[? ?] [?|?]]; [contradiction|]. apply (inter23 y).
+        by rewrite VSet.inter_spec.
+      - rewrite VSet.inter_spec VSet.add_spec. intros [[H0|?] ?]. 
+        + rewrite<- H0 in H.
+          apply (inter12 y). by rewrite VSet.inter_spec.
+        + apply (inter31 y). by rewrite VSet.inter_spec.
+    Qed.
+
+    Lemma partition_move_13 total v s l x : ~ VSet.In x v ->
+      Partition total (VSet.add x v) s (VSetProp.of_list l) ->
+      Partition total v s (VSetProp.of_list (x::l)).
+    Proof.
+      intros H [[=<-] [inter12 [inter23 inter31]]].
+      repeat split; [apply VSet.eq_leibniz| | |]; intro y.
+      - cbn. repeat rewrite VSet.union_spec. repeat rewrite VSet.add_spec.
+        split.
+        + by intros [?|[?|[?|?]]]; [left;right|right;left|left;left|right;right].
+        + by intros [[?|?]|[?|?]]; [right;right;left|left|right;left|right;right;right].
+      - rewrite VSet.inter_spec. intros [? ?]. apply (inter12 y).
+        rewrite VSet.inter_spec VSet.add_spec. by split; [right|].
+      - cbn. rewrite VSet.inter_spec VSet.add_spec. intros [? [H0|?]].
+        + apply (inter12 x). rewrite VSet.inter_spec VSet.add_spec. rewrite<- H0.
+          by split; [left|].
+        + apply (inter23 y). by rewrite VSet.inter_spec.
+      - cbn. rewrite VSet.inter_spec VSet.add_spec. intros [[H0|?] ?].
+        + apply H. by rewrite<- H0.
+        + apply (inter31 y). rewrite VSet.inter_spec VSet.add_spec.
+          by split; [|right].
+    Qed.
+
+    Lemma partition_in total v s l x : VSet.In x total ->
+      Partition total v s l -> VSet.In x v \/ VSet.In x s \/ VSet.In x l.
+    Proof.
+      intros H [H0 _]. rewrite<- H0 in H. revert H.
+      by repeat rewrite VSet.union_spec.
+    Qed.
+
+    Lemma aaa x y : (∑ n, In (x, n, y) (EdgeSet.elements (E G))) -> ∑ n, EdgeSet.In (x, n, y) (E G).
+    Proof.
+      intros [n Hn]. exists n. apply-> EdgeSet.elements_spec1.
+      apply InA_alt. by exists (x, n, y).
+    Qed.
+
+    Lemma aaaa x : forall y, In y (map (fun x => x.2) (succs G x)) -> Edges G x y.
+    Proof.
+      intros y Hy. apply aaa. unfold succs in Hy. revert y Hy.
+      induction (EdgeSet.elements (E G)).
+      - easy.
+      - simpl. intros y H. destruct (VSetDecide.F.eq_dec a..s x).
+        + cbn in H. destruct (V.eq_dec a..t y).
+          * exists (a..w). left. rewrite<- e0, <-e. destruct a as [[] ?].
+            reflexivity.
+          * destruct (IHl y) as [n0 ?].
+            -- destruct H; [contradiction|assumption].
+            -- exists (n0). by right.
+        + cbn in H. destruct (IHl y H) as [n0 ?]. exists n0. by right.
+    Qed.
+
+    Lemma aaaa_rev x y : Edges G x y -> In y (map (fun x => x.2) (succs G x)).
+    Proof.
+      intros [n e].
+      apply<- in_map_iff. exists (n, y). split; [reflexivity|].
+      apply<- in_map_iff. exists (x, n, y). split; [reflexivity|].
+      apply filter_In. split.
+      - apply EdgeSet.elements_spec1 in e as H1.
+        apply InA_alt in H1 as [y0 [H1 H2]].
+        now rewrite H1.
+      - cbn. destruct V.eq_equiv as [refl _ _].
+        destruct (VSetDecide.F.eq_dec x x); [reflexivity|].
+        now specialize (V.eq_leibniz x x (refl x)).
+    Qed.
+
+    Lemma inv_cardinal s x : VSet.In x s -> exists n, VSet.cardinal s = S n.
+    Proof.
+      intros [y [[=->] H%in_split]]%VSetFact.elements_1%InA_alt.
+      destruct H as [l1 [l2 H]]. rewrite VSet.cardinal_spec H app_length.
+      cbn. rewrite<- plus_n_Sm. by exists (#|l1| + #|l2|).
+    Qed.
+
+  End Stuff.
+
   Section topological_sort.
     Context (G:t).
     Context {HI : invariants G}.
@@ -70,10 +196,10 @@ Module WeightedGraphExt (V: UsualOrderedTypeWithLeibniz) (VSet : MSetList.SWithL
       | O => (l, s)
       | S n =>
         match VSet.mem x s with
-        | true => let (l', s') := (List.fold_left
+        | true => let a := (List.fold_left
             (fun a u => (topological_sort00 n a.2 a.1 u))
             (List.map (fun x => x.2) (succs G x)) (l,VSet.remove x s)) in
-            (x::l', s')
+            (x::a.1, a.2)
         | false => (l, s)
         end
       end.
@@ -98,17 +224,27 @@ Module WeightedGraphExt (V: UsualOrderedTypeWithLeibniz) (VSet : MSetList.SWithL
           etransitivity; eassumption.
     Qed.
 
+    Lemma topological_sort00_truc2 l1 : forall fuel a s',
+      VSet.Subset a.2 s' ->
+      VSet.Subset (fold_left (fun a u => (topological_sort00 fuel a.2 a.1 u))
+        l1 a).2 s'.
+    Proof.
+      induction l1 as [|x l1] => //.
+      intros fuel a s' H. cbn. apply IHl1.
+      transitivity a.2 => //. apply topological_sort00_truc.
+    Qed.
+
     Definition topological_sort0 s := topological_sort00 (VSet.cardinal s) s.
 
     Lemma topological_sort00_inc : forall m n s l x, m <= n -> VSet.cardinal s <= m ->
       topological_sort00 n s l x = topological_sort0 s l x.
     Proof.
       induction m.
-      - intros n s l x H HH. unfold topological_sort0, topological_sort00.
-        inversion HH. rewrite H1. case n => //. apply VSetProp.cardinal_inv_1 in H1.
-        specialize (H1 x). apply VSetProp.FM.not_mem_iff in H1.
+      - intros n s l x H HH. unfold topological_sort0.
+        inversion HH as [H1|H1]. rewrite H1. case n => //. apply VSetProp.cardinal_inv_1 in H1.
+        specialize (H1 x). apply VSetProp.FM.not_mem_iff in H1. cbn.
         now rewrite H1.
-      - intros. unfold topological_sort0.
+      - intros n s0 l x H H0. unfold topological_sort0.
         destruct n; [inversion H|].
         remember (S m) as m0.
         destruct H0; [|apply IHm; lia].
@@ -137,14 +273,21 @@ Module WeightedGraphExt (V: UsualOrderedTypeWithLeibniz) (VSet : MSetList.SWithL
       (l : list B) : forall a, P a -> (forall a0 b, P a0 -> f a0 b = g a0 b) ->
       (forall a0 b, P a0 -> P (f a0 b)) -> fold_left f l a = fold_left g l a.
     Proof.
-    Admitted.
+      induction l.
+      - cbn. reflexivity.
+      - cbn. intros a0 H H0 H1. rewrite<- (H0 a0 a H).
+        apply IHl.
+        + now apply H1.
+        + exact H0.
+        + exact H1.
+    Qed.
 
     Lemma topological_sort0_eq s l x: topological_sort0 s l x =
       match VSet.mem x s with
-      | true => let (l', s') := (List.fold_left
+      | true => let a := (List.fold_left
           (fun a u => (topological_sort0 a.2 a.1 u))
           (List.map (fun x => x.2) (succs G x)) (l, VSet.remove x s)) in
-          (x::l', s')
+          (x::a.1, a.2)
       | false => (l, s)
       end.
     Proof.
@@ -158,49 +301,287 @@ Module WeightedGraphExt (V: UsualOrderedTypeWithLeibniz) (VSet : MSetList.SWithL
         case_eq (VSet.mem x s); [|reflexivity].
         intro HH. rewrite<- (@VSetProp.remove_cardinal_1 s x) in H;
         [|now apply VSetFact.mem_iff]. inversion H as [H1].
-        rewrite H1. Check fold_left.
-    Admitted.
+        rewrite H1. rewrite (fold_left_ext _ 
+          (fun a u => topological_sort00 (VSet.cardinal a.2) a.2 a.1 u)
+          (fun a => VSet.cardinal a.2 <= fuel)).
+        + cbn. rewrite H1. apply le_n.
+        + intros a0 b H2. now apply (topological_sort00_inc (VSet.cardinal a0.2)).
+        + intros a0 b H2. transitivity (VSet.cardinal a0.2); [|assumption].
+          apply VSetProp.subset_cardinal. apply topological_sort00_truc.
+        + reflexivity.
+    Qed.
 
     Definition topological_sort := (topological_sort0 (V G) nil (s G)).1.
 
     Lemma topological_sort0_set_eq {s s' x} :
       VSet.Equal s s' -> topological_sort0 s x = topological_sort0 s' x.
     Proof.
-      intro H. unfold topological_sort0. rewrite (VSetProp.Equal_cardinal H).
-      set (n := VSet.cardinal s').
-      clearbody n. revert s s' x H. induction n.
-      - reflexivity.
-      - unfold topological_sort00. intros s s' x H.
-        rewrite (VSet.eq_leibniz H). reflexivity.
+      intros [=->]%VSet.eq_leibniz. reflexivity.
+    Qed.
+
+    Lemma topological_sort00_bla fuel s l x : exists l', (topological_sort00 fuel s l x).1 = l' ++ l.
+    Proof.
+      revert x l s.
+      induction fuel.
+      - exists []. now cbn.
+      - intros x l s.
+        cbn. destruct (VSet.mem x s).
+        + set l2 := map _ _. clearbody l2. cbn. set p := (l, VSet.remove x s).
+          assert (exists l', p.1 = l' ++ l) as H; [exists [] ;reflexivity|]. revert H. generalize p.
+          induction l2.
+          * cbn. intros p0 [l' H]. rewrite H. exists (x :: l'). reflexivity.
+          * cbn. intros p0 [l' H]. apply (IHl2 (topological_sort00 fuel p0.2 p0.1 a)).
+            destruct (IHfuel a p0.1 p0.2) as [l'' H0].
+            exists (l'' ++ l'). rewrite<- app_assoc. rewrite H0. now rewrite H.
+        + exists []. reflexivity.
+    Qed.
+
+    Lemma topological_sort00_blabla fuel s l l2 : exists l', (fold_left (fun a u => topological_sort00 fuel a.2 a.1 u) l2 (l, s)).1 = l' ++ l.
+    Proof.
+      revert fuel s l.
+      induction l2.
+      - cbn. by exists [].
+      - cbn. intros fuel s l. destruct (topological_sort00_bla fuel s l a) as [l'' H].
+        set p := topological_sort00 _ _ _ _. destruct (IHl2 fuel p.2 p.1) as [l' H0].
+        exists (l' ++ l''). rewrite<- app_assoc. rewrite<- (surjective_pairing p) in H0.
+        rewrite H0. unfold p, topological_sort0. now rewrite H.
+    Qed.
+
+    Definition topological_sort0_bla s l x : exists l', (topological_sort0 s l x).1 = l' ++ l :=
+      topological_sort00_bla (VSet.cardinal s) s l x.
+
+    Definition topological_sort0_blabla s l l2 : exists l', (fold_left (fun a u => topological_sort0 a.2 a.1 u) l2 (l, s)).1 = l' ++ l.
+    Proof.
+      destruct (topological_sort00_blabla (VSet.cardinal s) s l l2) as [l' H].
+      exists l'. rewrite<- H. set fa := fold_left _ _ _. set fb := fold_left _ _ _.
+      enough (fa = fb).
+      + by rewrite H0.
+      + unfold fa, fb. apply (fold_left_ext _ _ (fun a => VSet.Subset a.2 s )); try easy.
+        * intros a b H0. symmetry. apply (topological_sort00_inc (VSet.cardinal s)).
+          - apply le_n.
+          - now apply VSetProp.subset_cardinal.
+        * intros a b H0. transitivity a.2; [|assumption]. apply topological_sort00_truc.
+    Qed.
+
+    Lemma topological_sort0_diet fuel s l x z : VSet.In z s -> ~ In z (topological_sort00 fuel s l x).1 ->
+      VSet.In z (topological_sort00 fuel s l x).2.
+    Proof.
+      revert s l x. induction fuel.
+      - easy.
+      - cbn. intros s l x. destruct (VSet.mem x s); [|easy].
+        set l' := map _ _. cbn. intros H [H0 H1]%not_in_cons.
+        assert (forall l'' p, VSet.In z p.2 -> ~ In z (fold_left (fun a u => topological_sort00 fuel a.2 a.1 u) l'' p).1->
+          VSet.In z (fold_left (fun a u => topological_sort00 fuel a.2 a.1 u) l'' p).2) as H2.
+        + induction l''.
+          * easy.
+          * cbn. intros p H2 H3. apply IHl''; [|assumption].
+            apply IHfuel; [assumption|]. remember (topological_sort00 _ _ _ _) as p0. destruct (topological_sort00_blabla fuel p0.2 p0.1 l'') as [l0 H4].
+            rewrite<- surjective_pairing in H4. rewrite H4 in H3.
+            intro. apply H3. apply in_or_app. right. assumption.
+        + apply H2; [now apply VSet.remove_spec|easy].
+    Qed.
+
+    Definition acyclic := forall x y, Edges G x y -> Paths G y x -> False.
+
+    Inductive is_topo_sorted : list V.t -> Prop :=
+      | is_topo_sorted_nil : is_topo_sorted []
+      | is_topo_sorted_cons x l : (forall y, Paths G x y -> In y (x::l)) -> is_topo_sorted l -> is_topo_sorted (x::l).
+
+    Lemma is_topo_sorted_alt l : is_topo_sorted l <->
+      (forall x y l1 l2, l = l1 ++ x :: l2 -> Paths G x y -> In y (x::l2)).
+    Proof.
+      split.
+      - intros H x0 y l1 l2 H1 p. revert l H H1. induction l1.
+        + intros l H H1. induction H.
+          * contradiction (app_cons_not_nil [] l2 x0 H1).
+          * injection H1. intros [=->] [=->]. apply H => //.
+        + intros l H H1. rewrite<- app_comm_cons in H1. rewrite H1 in H.
+          inversion H as [|x l0 H0 H2 [H3 H4]]. apply (IHl1 (l1 ++ x0 :: l2)) => //.
+      - intros H. induction l; [constructor|].
+        constructor.
+        + intros y p. apply (H _ _ []) => //.
+        + apply IHl. intros x y l1 l2 H0 p. apply (H _ _ (a::l1)) => //.
+          rewrite<- app_comm_cons. by rewrite H0.
+    Qed.
+
+    Lemma is_topo_sorted_weak l y z : is_topo_sorted l -> In y l ->
+      Paths G y z -> In z l.
+    Proof.
+      intros H [l1 [l2 H0]]%in_split p. rewrite H0 in H |- *. clear H0.
+      induction l1.
+      - inversion H. apply H2 => //.
+      - rewrite<- app_comm_cons. apply in_cons. apply IHl1. inversion H => //.
+    Qed.
+
+    Lemma union_add_remove x s s' : VSet.In x s ->
+      VSet.union (VSet.add x s') (VSet.remove x s) = VSet.union s' s.
+    Proof.
+      intro. apply VSet.eq_leibniz. intro a.
+      repeat rewrite VSet.union_spec. rewrite VSet.add_spec VSet.remove_spec.
+      split.
+      - intros [[?|?]|[? ?]].
+        + rewrite H0. by right.
+        + by left.
+        + by right.
+      - intros [?|?].
+        + by left; right.
+        + destruct (V.eq_dec a x) as [[=->]|H1].
+          * by left; left.
+          * right. by split.
+    Qed.
+
+    Lemma union_add x s s' : VSet.union (VSet.add x s) s' = VSet.add x (VSet.union s s').
+    Proof.
+      apply VSet.eq_leibniz. intro a.
+      rewrite VSet.union_spec VSet.add_spec VSet.add_spec VSet.union_spec.
+      split.
+      - by intros [[?|?]|?]; [left|right;left|right;right].
+      - by intros [?|[?|?]]; [left;left|left;right|right].
+    Qed.
+
+    Definition configuration v s l x : Prop := Partition (V G) v s (VSetProp.of_list l) /\
+      (forall y, Paths G x y -> VSet.In y v -> False) /\ is_topo_sorted l.
+
+    Definition config' v s l : Prop := Partition (V G) v s (VSetProp.of_list l) /\
+      is_topo_sorted l.
+
+    Lemma config_init : configuration VSet.empty (V G) [] (s G).
+    Proof.
+      repeat split; cbn; have Hempty := VSet.empty_spec.
+      - rewrite (VSet.eq_leibniz (VSetProp.empty_union_1 _ _)) => //.
+        rewrite (VSet.eq_leibniz (VSetProp.empty_union_2 _ _)) => //.
+      - apply VSetProp.empty_inter_1 => //.
+      - apply VSetProp.empty_inter_2 => //.
+      - apply VSetProp.empty_inter_1 => //.
+      - intros ? _ ?%VSetFact.empty_1 => //.
+      - constructor.
+    Qed.
+
+(*
+    Lemma truc fuel x : 
+      forall l0 l1 v s l, map (fun x => x.2) (succs G x) = l1 ++ l0 ->
+      let a := fold_left (fun a u => topological_sort00 fuel a.2 a.1 u)
+        l1 (l, s) in configuration v a.2 a.1 x -> 
+      let a := fold_left (fun a u => topological_sort00 fuel a.2 a.1 u)
+        (l1 ++ l0) (l, s) in configuration v a.2 a.1 x.
+    Proof.
+      intro l0. induction l0.
+      - intros l1 v s l H. by rewrite (app_nil_r l1).
+      - intros l1 v s0 l H. assert (l1 ++ a :: l0 = (l1 ++ [a]) ++ l0) as H0.
+        + by rewrite<- app_assoc.
+        + intros a0 Hl1. rewrite H0. apply IHl0; [easy|].
+          rewrite fold_left_app. fold a0. cbn.
+    Admitted.
+*)
+    Definition succ' x := map (fun x => x.2) (succs G x).
+
+    Context {Ha : acyclic}.
+
+    Lemma violent fuel : forall v s l x, configuration v s l x ->
+      VSet.cardinal s <= fuel ->
+      let a := (topological_sort00 fuel s l x) in configuration v a.2 a.1 x.
+    Proof.
+      induction fuel => //.
+      intros v s l x config Hfuel.
+      destruct config as [part [back_path topo_sort]]. cbn delta fix match beta.
+      destruct (VSet.mem x s) eqn: H0 => //.
+      apply VSetFact.mem_iff in H0.
+      set l0 := succ' x.
+      assert (succ' x = [] ++ l0) as H => //.
+      assert (let a := fold_left (fun a u => topological_sort00 fuel a.2 a.1 u)
+        [] (l, VSet.remove x s) in config' (VSet.add x v) a.2 a.1 /\
+          forall y z, Edges G x y -> In y [] -> Paths G y z -> In z (x::a.1)).
+      - split => //. split => //. apply partition_move_21 => //.
+      - fold (succ' x). rewrite H. elim: l0 [] H H1.
+        + intro l1. rewrite app_nil_r. intros H [[? ?] ?].
+          split; [|split] => //.
+          * apply partition_move_13 => //. destruct part as [_ [part _]].
+            intro. apply (part x). by rewrite VSet.inter_spec.
+          * constructor => //.
+            intros y path. destruct path; [apply in_eq|].
+               apply (H3 y) => //. rewrite<- H. apply aaaa_rev => //.
+        + intros x0 l0 IHl0 l1. set a := fold_left (fun a0 u => topological_sort00 fuel a0.2 a0.1 u) l1
+            (l, VSet.remove x s).
+          intros H [[Hpart Hsorted] Hpath].
+          assert (l1 ++ x0 :: l0 = (l1 ++ [x0]) ++ l0) as H2; [by rewrite<- app_assoc|].
+          rewrite H2. apply IHl0; [easy|].
+          rewrite fold_left_app. fold a. cbn.
+          destruct (IHfuel (VSet.add x v) a.2 a.1 x0) as [? [? ?]]; [| |split => //].
+          * split; [|split] => //. intros y path [Hy|Hy]%VSet.add_spec.
+            -- rewrite Hy in path. unfold acyclic in Ha. apply (Ha x x0) => //.
+               apply aaaa. fold (succ' x). rewrite H. apply in_or_app. right.
+               apply in_eq.
+            -- apply (back_path y) => //. apply (paths_step _ _ x0); [|eassumption].
+               apply aaaa. fold (succ' x). rewrite H. apply in_or_app. right. apply in_eq.
+          *  assert (S (VSet.cardinal (VSet.remove x s)) = VSet.cardinal s) as H6;
+              [apply VSetProp.remove_cardinal_1 => //|].
+            rewrite<- H6 in Hfuel. apply le_S_n in Hfuel.
+            transitivity (VSet.cardinal (VSet.remove x s)) => //.
+            apply VSetProp.subset_cardinal. apply topological_sort00_truc2.
+            apply VSetProp.subset_refl.
+          * intros y z e [Hy|[[=->]|?]]%in_app_or p => //.
+            -- destruct (Hpath y z e Hy p); [by left|]. right.
+               destruct (topological_sort00_bla fuel a.2 a.1 x0) as [? [=->]].
+               apply in_or_app. by right.
+            -- right. destruct HI as [edges _ _]. specialize (edges _ e.π2) as [_ Iny].
+               cbn in Iny.
+               destruct (partition_in _ _ _ _ _ Iny H1) as [[H5%V.eq_leibniz|H5]%VSet.add_spec|[H5|H5]].
+               ++ exfalso. unfold acyclic in Ha. apply (Ha x y) => //. rewrite H5.
+                  apply paths_refl.
+               ++ exfalso. apply (back_path y) => //.
+                  apply (paths_step _ _ y) => //. apply paths_refl.
+               ++ assert (S (VSet.cardinal (VSet.remove x s)) = VSet.cardinal s) as H6;
+                    [apply VSetProp.remove_cardinal_1 => //|].
+                  rewrite<- H6 in Hfuel. apply le_S_n in Hfuel.
+                  assert (VSet.In y a.2); [apply (topological_sort00_truc a.1 y fuel a.2) => //|].
+                  assert (VSet.Subset a.2 (VSet.remove x s)).
+                  1: {apply topological_sort00_truc2. apply VSetProp.subset_refl. }
+                  assert (VSet.cardinal a.2 <= fuel). 
+                  1: {transitivity (VSet.cardinal (VSet.remove x s)) => //. apply VSetProp.subset_cardinal => //. }
+                  destruct (inv_cardinal a.2 y) as [n H10] => //. rewrite H10 in H9.
+                  destruct fuel; [inversion H9|]. apply (is_topo_sorted_weak _ y) => //.
+                  cbn. apply (VSetFact.mem_iff a.2 y) in H7 as [=->]. apply in_eq.
+               ++ apply (is_topo_sorted_weak _ y) => //. revert H5.
+                  rewrite VSetProp.of_list_1. by intros [? [[=->] ?]]%InA_alt.
+    Qed.
+
+    Lemma machin x z v s l: Paths G x z -> VSet.In x s ->
+      configuration v s l x -> In z (topological_sort0 s l x).1.
+    Proof.
+      intros p H%VSetFact.mem_iff config.
+      apply (violent (VSet.cardinal s)) in config => //.
+      destruct config as [_ [_ ?]].
+      apply (is_topo_sorted_weak _ x) => //. rewrite topological_sort0_eq H.
+      apply in_eq.
     Qed.
 
     Lemma topological_sort0_in y: VSet.In y (V G) ->
       In y (topological_sort).
     Proof.
-      intro H. unfold topological_sort. rewrite topological_sort0_eq.
-      destruct HI as [edges_vertices [=->]%VSetFact.mem_iff source_paths].
-      specialize (source_paths y H) as [[x _]]. induction x.
-      - apply in_eq.
-      - apply in_cons. destruct e as [n e].
-        assert (In y (map (fun x1 : Z × V.t => x1.2) (succs G x))).
-        + apply<- (in_map_iff).
-          exists (n, y). split; [now cbn|].
-          apply<- (in_map_iff).
-          exists (x, n, y). split; [now cbn|].
-          apply filter_In.
-          split. apply EdgeSet.elements_spec1 in e.
-          apply InA_alt in e. destruct e as [y0 [H0 H1]].
-          now rewrite H0. cbn. destruct (VSetDecide.F.eq_dec x x); [now cbn|].
-          destruct V.eq_equiv as [refl _ _]. now specialize (V.eq_leibniz x x (refl x)) as H0.
-        + apply in_split in H0 as [l1 [l2 [=->]]]. rewrite fold_left_app.
-
+      intro H. destruct HI as [edges source path].
+      apply (machin _ _ VSet.empty) => //.
+      - admit.
+      - apply config_init.
     Admitted.
 
-    Lemma topological_sort0_spec s x l l': topological_sort = l ++ x::l' ->
-      SortFamilySet.For_all (fun x' => is_eliminable constraints x x' -> In x' l') (sGraph.V local_graph).
+    Lemma topological_sort0_spec x l l': topological_sort = l ++ x::l' ->
+      forall y, Paths G x y -> In y (x::l').
     Proof.
+      intros H y p.
+      have config := config_init. apply (violent (VSet.cardinal (V G))) in config => //.
+      destruct config as [_ [_ is_sorted]].
+      destruct (is_topo_sorted_alt topological_sort) as [H0 _].
+      apply (H0 is_sorted x y l l' H p).
+    Qed.
+
+  Definition pred (x : V.t) : list V.t := 
+    let l := List.filter (fun e => V.eq_dec e..t x) (EdgeSet.elements (E G)) in
+    List.map (fun e => e..s) l.
   End topological_sort.
-End sGraph.
+
+End WeightedGraphExt.
+
+Module Import sGraph := WeightedGraphExt SortFamily SortFamilySet.
 
 Definition add_sorts : SortConstraint.t -> SortFamilySet.t -> SortFamilySet.t :=
   fun c s => SortFamilySet.add c.2 (SortFamilySet.add c.1 s).
@@ -606,11 +987,46 @@ Section GoodConstraints.
   Definition global_local_agreement: bool := SortFamilySet.for_all
     (fun s => SortFamilySet.for_all (fun s' => respect_constraints s s') global_sorts) global_sorts.
 
+  Definition assignment : Set := list (nat × SortFamily.t).
+  Definition get_value (ρ : assignment) (s : SortFamily.t) : option SortFamily.t :=
+    match s with
+    | SortFamily.sfVar n => match find (fun p => Nat.eqb p.1 n) ρ with
+      | None => None
+      | Some (m, s') => Some s'
+      end
+    | _ => Some s
+    end.
 
-  Fixpoint assign_variables (x:SortFamily.t) (ρ: valuation) (fuel: nat): option valuation :=
-    match fuel with
-      | O => None
-      | S n =>
+  Fixpoint gather_option (l : list (option (SortFamily.t))) : option SortFamilySet.t :=
+    match l with
+    | [] => Some SortFamilySet.empty
+    | None :: l' => None
+    | Some s :: l' => match gather_option l' with
+      | None => None
+      | Some sfSet => Some (SortFamilySet.add s sfSet)
+      end
+    end.
+
+  Definition join_option (l : option (SortFamilySet.t)) : option SortFamily.t :=
+    match l with
+    | None => None
+    | Some s => join s
+    end.
+
+  Fixpoint assign_variables (ρ: assignment) (vertices: list SortFamily.t): option assignment :=
+    match vertices with
+    | [] => Some ρ
+    | sort :: l => match sort with
+      | SortFamily.sfVar n => 
+        match gather_option (map (get_value ρ) (pred local_graph (sort))) with
+        | None => None
+        | Some preds => match join preds with
+          | None => None
+          | Some sort => assign_variables ((n, sort)::ρ) l
+          end
+        end 
+      | _ => assign_variables ρ l
+      end
     end.
 
   Definition constraints_correct
